More fiddlign with defns

src/Find_proof.thy
@@ -4,14 +4,10 @@ begin
 
 (*begin find invariant*)
 definition invariant_wf_fts :: "bool" where
-"invariant_wf_fts = (
-  total_order_key_lte --> (
-  ! fts.
-  let wellformed_fts' = (
-    let fts' = step_fts fts in
-    case fts' of None => True | Some fts' => wellformed_fts fts')
-  in
- wellformed_fts fts --> wellformed_fts'))
+"invariant_wf_fts = (! fts fts'.
+  total_order_key_lte &
+  (step_fts fts = Some (fts')) &
+  wellformed_fts fts \<longrightarrow> wellformed_fts fts')
 "
 (*end find invariant*)
 
@@ -29,7 +25,9 @@ done
 
 declare  wellformed_context.simps[simp del]
 
+(*
 declare wellformed_context_def_2[simp del] (* not a simp? - may expand too far? or use anyway? *)
+*)
 
 declare ts_to_ms_def_2[simp] (* likely a simp *)
 declare dest_fts_state_t_def_2[simp] (* surely a simp *)
@@ -58,16 +56,10 @@ apply(force intro: FIXME)
 done
 
 lemma lu_with_default_eq_lu: "
-min_child_index < i &
-i < max_child_index(ks,rs) \<longrightarrow>
-get_lu_for_child_with_parent_default x2 ((ks,rs),i) = get_lu_for_child ((ks,rs),i)"
+min_child_index < i & i < max_child_index(ks,rs) 
+\<longrightarrow> (get_lu_for_child_with_parent_default x2 ((ks,rs),i) = get_lu_for_child ((ks,rs),i))"
 apply(force intro:FIXME)
 done
-
-(*
-wellformed_fts_focus (ts_to_ms ts) (Node (ks, rs)) \<Longrightarrow>
-       wellformed_context ts \<Longrightarrow>
-*)
 
 lemma get_parent_bounds_check_keys: "
 wellformed_fts_1 (Fts_state (k, Node (ks, rs), ts)) \<Longrightarrow>
@@ -83,6 +75,8 @@ apply(simp add: wellformed_fts_1_def dest_cnode_t_def)
 apply(force simp add: check_keys_def)
 done
 
+
+(* FIXME do we also want to include keys(rs!i) in the bound? *)
 definition main_property :: "fts_state_t \<Rightarrow> bool" where
 "main_property fts' = (
   let (k,t,ts) = dest_fts_state_t fts' in
@@ -95,9 +89,9 @@ definition main_property :: "fts_state_t \<Rightarrow> bool" where
   ))"
 
 lemma main_lemma: "(
-(* want to check_keys l [k] u *)
-total_order_key_lte --> (
-  wellformed_fts fts & (step_fts fts = Some fts') --> main_property fts'))
+total_order_key_lte &
+(step_fts fts = Some fts') &
+wellformed_fts fts --> main_property fts')
 "
 apply(simp add: main_property_def)
 apply(simp, intro allI impI, elim conjE)
@@ -132,26 +126,30 @@ apply(rule conjI)
   (* min_child_index < i *)
   apply(force intro:FIXME)
 
- (* want check_keys None [k] u0 *)
+  (* want check_keys None [k] u0 *)
   apply(subgoal_tac "? l1 u1. get_parent_bounds ts = (l1,u1)") prefer 2 apply(force intro:FIXME)
   apply(elim exE,simp)
-  apply(subgoal_tac "u0 = u1") prefer 2 apply(force intro:FIXME)
-  apply(simp)
-  apply(simp add: wellformed_fts_def ) apply(elim conjE)
-  using check_keys_eq_ck_ck get_parent_bounds_check_keys apply blast
+  apply(subgoal_tac "(i = max_child_index(ks,rs)) | (min_child_index \<le> i & i < max_child_index(ks,rs))") prefer 2 apply(force intro:FIXME)
+  apply(elim disjE)
+  
+   apply(subgoal_tac "u0 = u1") prefer 2 apply(force intro:FIXME)
+   apply(simp)
+   apply(simp add: wellformed_fts_def ) apply(elim conjE)
+   using check_keys_eq_ck_ck get_parent_bounds_check_keys apply blast
+
+   (* i < max_child_index *)
+   apply(force intro: FIXME)
 done 
 
 
 (* intuitively, we examine all the possible cases... *)
-lemma invariant_wf_fts: "invariant_wf_fts"
+lemma invariant_wf_fts: "
+  invariant_wf_fts
+"
 apply (simp add:invariant_wf_fts_def)
 apply(intro impI allI)
-apply(subgoal_tac "(step_fts fts = None) | (? fts'. step_fts fts = Some(Fts_state(fts')))")
-  prefer 2 apply(force intro:FIXME)
-apply(erule disjE) apply(force)
-apply(elim exE)
-apply(simp)
-apply(subgoal_tac "main_property (Fts_state(fts'))")
+apply(elim exE conjE)
+apply(subgoal_tac "main_property fts'")
  prefer 2 apply (simp add: main_lemma option.case_eq_if)
 apply(simp add: step_fts_def)
 apply(subgoal_tac "? k t ts. fts = Fts_state(k,t,ts)") prefer 2 apply(force intro: FIXME)
@@ -163,16 +161,12 @@ apply(erule disjE)
 
  (* t = Node(ks,rs) *)
  apply(elim exE, simp)
+ apply(thin_tac "t=_")
  apply(subgoal_tac "? i. search_key_to_index ks k = i") prefer 2 apply(force)
  apply(elim exE, simp)
  apply(subgoal_tac "
-   ? xtra. (get_lu_for_child_with_parent_default (get_parent_bounds ts) ((ks, rs), i) = xtra)") prefer 2 apply(force)
+   ? l0 u0. (get_lu_for_child_with_parent_default (get_parent_bounds ts) ((ks, rs), i) = (l0,u0))") prefer 2 apply(force)
  apply(elim exE, simp)
- apply(subgoal_tac "? l0 u0. xtra = (l0,u0)") prefer 2 apply(force intro: FIXME)
- apply(elim exE)
- apply(simp)
- apply(thin_tac "t=_")
- apply(thin_tac "xtra = _")
  apply(subgoal_tac "i : set(subtree_indexes (ks,rs))") prefer 2 apply(force intro:FIXME)
  apply(subgoal_tac "? r. r : set(rs) &  (rs ! i) = r") prefer 2 apply(force intro:FIXME)
  apply(elim exE conjE, simp)
@@ -194,14 +188,22 @@ apply(erule disjE)
    (* want wellformed_tree *)
    apply(force simp add: wellformed_fts_focus_def)
 
-   (* check_keys l0 (keys r) u0 ; suppose pb is a bound for rs, then lget_lu_with_def is a bound for rs!i *)
+   (* check_keys l0 (keys r) u0 ; suppose pb is a bound for rs, then lget_lu_with_def is a bound for rs!i 
+   we also need that all keys of t are bounded by the parent l0 u0; but we have this from the 
+   previous step, wf_fts_1? except it doesn't in case we are extremal
+   *)
    apply(force intro: FIXME)
+
+  (* FIXME search key to index should take some existing bounds, and return new bounds as well? get_lu_for_child is then search_key_to_index 
+  perhaps it is worth incorporating the bound into the focus?
+
+ *)
+
 
   (* want wellformed_fts_1 k,r,cn1#ts *)
   apply(simp (no_asm) add: wellformed_fts_1_def dest_fts_state_t_def dest_cnode_t_def)
   apply(simp)
   (* want check_keys l0 [k] u0 this comes from the fact that k is the search key, and this is bounded *)
-  (* FIXME need lemma about get_lu_for_child *)
   apply(force simp add: main_property_def dest_cnode_t_def)
 
 done
