src/Tree_stack.thy
@@ -1,46 +1,56 @@
 theory Tree_stack imports Tree begin
 
-type_synonym xtra_t = "(key option * key option)"  (* l,u *)
+(* the bound is a bound on ALL children, not just rs!i *)
+datatype cnode_t = Cnode "node_t * nat * bound_t"  (* n,i,b *)
 
-datatype cnode_t = Cnode "node_t * nat * xtra_t"  (* n,i,x *)
-definition dest_cnode_t :: "cnode_t \<Rightarrow> node_t * nat * xtra_t" where
-"dest_cnode_t c = (case c of Cnode (n,i,x) \<Rightarrow> (n,i,x))"
+
+definition dest_cnode_t :: "cnode_t \<Rightarrow> node_t * nat * bound_t" where
+"dest_cnode_t c = (case c of Cnode (n,i,b) \<Rightarrow> (n,i,b))"
 
 (* FIXME remove *)
 type_synonym context_t = "cnode_t list"
 
 type_synonym tree_stack_t = "cnode_t list"
 
-(* wellformed_context ---------------------------------------- *)
 
-definition get_parent_bounds :: "context_t \<Rightarrow> xtra_t" where
+
+
+(* bound from cnode ---------------------------------------- *)
+
+(* make sure we use the existing bound in case i is extremal *)
+definition cnode_to_bound :: "cnode_t \<Rightarrow> bound_t" where
+"cnode_to_bound cn = (
+  let (n,i,b) = dest_cnode_t cn in
+  let (ks,rs) = n in
+  index_to_bound ks i |> with_parent_bound b)"
+
+
+(* bound from tree stack ---- *)
+
+(* FIXME disappears ?*)
+(*
+definition get_parent_bounds :: "context_t \<Rightarrow> bound_t" where
 "get_parent_bounds ts = (
   case ts of 
   Nil \<Rightarrow> (None,None)
   | cn#_ \<Rightarrow> (let (n,i,x) = dest_cnode_t cn in x))"
+*)
 
 
-(* version of get_lu if parent bound is known *)
-definition get_lu_for_child_with_parent_default :: "xtra_t \<Rightarrow> (node_t*nat) \<Rightarrow> xtra_t" where
-"get_lu_for_child_with_parent_default x2 ni = (
-  let (l1,u1) = get_lu_for_child ni in
-  let (l2,u2) = x2 in
-  let l = (case l1 = None of True \<Rightarrow> l2 | _ \<Rightarrow> l1) in
-  let u = (case u1 = None of True \<Rightarrow> u2 | _ \<Rightarrow> u1) in
-  (l,u)
-)"
+(* wellformed_cnode ---------------------------------------- *)
+
+
 
 (* FIXME adjust scala defns *)      
-definition wellformed_cnode :: "ms_t => xtra_t \<Rightarrow> cnode_t => bool " where
-"wellformed_cnode ms x2 cn = (
+definition wellformed_cnode :: "ms_t => cnode_t => bool " where
+"wellformed_cnode ms cn = (
   let (n1,i1,x1) = dest_cnode_t cn in 
+  let (l1,u1) = x1 in
   let (ks,rs) = n1 in
   let b1 = wellformed_tree ms (Node(ks,rs)) in  (* FIXME wellformed_kv_tree *)
   let b2 = i1 : set(subtree_indexes (ks,rs)) in
-  let (l1,u1) = x1 in
-  let b3 = check_keys l1 (keys (rs!i1)) u1 in
-  let b4 = (x1 = get_lu_for_child_with_parent_default x2 (n1,i1)) in
-  b1&b2&b3&b4)
+  let b3 = check_keys l1 (keys (Node(ks,rs))) u1 in
+  b1&b2&b3)
 "
 
 definition ts_to_ms :: "tree_stack_t \<Rightarrow> ms_t" where
@@ -52,62 +62,20 @@ lemma ts_to_ms_def_2: "
   apply(simp add:ts_to_ms_def)
   done
 
+
+(* wellformed_context ---------------------------------------- *)
+
+
 fun wellformed_context :: "context_t => bool" where
 "wellformed_context xs = (
   case xs of Nil \<Rightarrow> True
-  | cn#cns \<Rightarrow> (
-    let ms = ts_to_ms cns in
-    let x2 = get_parent_bounds cns in
-    wellformed_cnode ms x2 cn & 
-    wellformed_context cns))"
+  | cn#cns \<Rightarrow> (wellformed_cnode (ts_to_ms cns) cn & wellformed_context cns))"
 (*end wfcontext definition*)
 
 lemma wellformed_context_def_2: "
   (wellformed_context  Nil = True) &
-  (wellformed_context (cn#cns) = (   
-    let ms = ts_to_ms cns in
-    let x2 = get_parent_bounds cns in
-    wellformed_cnode ms x2 cn & 
-    wellformed_context cns))"
+  (wellformed_context (cn#cns) = (wellformed_cnode (ts_to_ms cns) cn & wellformed_context cns))"
 by simp
-
-(* old ---------------------------------------- *)
-
-(* old defintiions? *)
-
-definition ctx_to_map :: "context_t => (key,value_t) map" where
-"ctx_to_map ctx == (
-let leaves = List.map (% cn. let (n,i,x) = dest_cnode_t cn in List.concat(tree_to_leaves (Node(n)))) ctx in
-map_of(List.concat leaves))"
-
-(* FIXME tr: above should use tree to map fun *)
-
-(* FIXME tr: use tree_stack_t for context_t *)
-
-
-(* FIXME move elsewhere *)
-(*begin focus definition*)
-datatype 'f focus_t = Focus 'f
-(*end focus definition*)
-
-
-
-(*begin treestack definition*)
-datatype 'f tree_stack = Tree_stack "'f focus_t * context_t"
-(*end treestack definition*)
-
-definition is_subnode 
- :: "node_t => (node_t * nat) => bool"
-where
-"is_subnode n pi == (
-  let ((ks,rs),i) = pi in
-  Node n = (rs!i))"
-
-(* FIXME in above, make sure is is an index *)
-
-
-definition dest_ts :: "'f tree_stack => 'f * context_t" where
-"dest_ts ts == (case ts of Tree_stack((Focus f),c) => (f,c))"
 
 
 end
